lib/crunch: monad predicate for instance interface
Instead of a function that returns the state part of the monad type, use
a predicate that says whether the given type is the instance monad or
not. This generalises instances to any monad type and avoids problems
when the concept of state is more complex such as in the environment
monad.

Signed-off-by: Gerwin Klein <gerwin.klein@proofcraft.systems>

lib/test/Crunch_Test_NonDet.thy
@@ -14,13 +14,13 @@ begin
 
 text \<open>Test cases for crunch\<close>
 
-definition
-  "crunch_foo1 (x :: nat) \<equiv> do
-    modify ((+) x);
-    modify ((+) x)
+definition crunch_foo1 :: "nat \<Rightarrow> (unit, nat, unit) nondet_monad" where
+  "crunch_foo1 x \<equiv> do
+    modify (map_state ((+) x));
+    modify (map_state ((+) x))
   od"
 
-definition
+definition crunch_foo2 :: "(unit, nat, unit) nondet_monad" where
   "crunch_foo2 \<equiv> do
     crunch_foo1 12;
     crunch_foo1 13
@@ -34,7 +34,7 @@ crunch crunch_foo2
 crunch_ignore (add: crunch_foo1)
 
 crunch crunch_foo2
-  for gt: "\<lambda>x. x > y"
+  for gt: "\<lambda>x. mstate x > y"
   (ignore_del: crunch_foo1)
 
 crunch_ignore (del: crunch_foo1)
@@ -66,12 +66,12 @@ crunch crunch_foo2
   for (valid) at_2: "crunch_always_true 2"
   (wp: crunch_foo1_at_2[simplified])
 
-fun crunch_foo3 :: "nat => nat => 'a => (nat,unit) nondet_monad" where
+fun crunch_foo3 :: "nat => nat => 'a => (unit, nat, unit) nondet_monad" where
   "crunch_foo3 0 x _ = crunch_foo1 x"
 | "crunch_foo3 (Suc n) x y = crunch_foo3 n x y"
 
 crunch crunch_foo3
-  for gt2: "\<lambda>x. x > y"
+  for gt2: "\<lambda>x. mstate x > y"
 
 crunch crunch_foo3
   for (empty_fail) empty_fail2
@@ -85,7 +85,7 @@ class foo_class =
   fixes stuff :: 'a
 begin
 
-fun crunch_foo4 :: "nat => nat => 'a => (nat,unit) nondet_monad" where
+fun crunch_foo4 :: "nat => nat => 'a => (unit, nat, unit) nondet_monad" where
   "crunch_foo4 0 x _ s = crunch_foo1 x s"
 | "crunch_foo4 (Suc n) x y s = crunch_foo4 n x y s"
 
@@ -102,18 +102,18 @@ lemma crunch_foo4_alt:
 
 (* prove rules about crunch_foo4 with and without the alternative definition *)
 crunch crunch_foo4
-  for gt3: "\<lambda>x. x > y"
+  for gt3: "\<lambda>x. mstate x > y"
 
 crunch crunch_foo4
   for (no_fail) no_fail2
   (rule: crunch_foo4_alt)
 
 crunch crunch_foo4
-  for gt3': "\<lambda>x. x > y"
+  for gt3': "\<lambda>x. mstate x > y"
   (rule: crunch_foo4_alt)
 
 crunch crunch_foo5
-  for gt4: "\<lambda>x. x > y"
+  for gt4: "\<lambda>x. mstate x > y"
 
 (* Test cases for crunch in locales *)
 
@@ -123,7 +123,7 @@ definition
 crunch_ignore (del: bind)
 
 locale test_locale =
-fixes fixed_return_unit :: "(unit, unit) nondet_monad"
+fixes fixed_return_unit :: "(unit, unit, unit) nondet_monad"
 
 begin
 
@@ -145,17 +145,17 @@ definition
 
 definition
   "crunch_foo9 (x :: nat) \<equiv> do
-    modify ((+) x);
-    modify ((+) x)
+    modify (map_state ((+) x));
+    modify (map_state ((+) x))
   od"
 
 crunch crunch_foo9
-  for test: "\<lambda>x. x > y" (ignore: bind)
+  for test: "\<lambda>x. mstate x > y" (ignore: bind)
 
 definition
   "crunch_foo10 (x :: nat) \<equiv> do
-    modify ((+) x);
-    modify ((+) x)
+    modify (map_state ((+) x));
+    modify (map_state ((+) x))
   od"
 
 (*crunch_def attribute overrides definition lookup *)
@@ -166,13 +166,13 @@ lemma crunch_foo10_def2[crunch_def]:
   by simp
 
 crunch crunch_foo10
-  for test[wp]: "\<lambda>x. x > y"
+  for test[wp]: "\<lambda>x. mstate x > y"
 
 (* crunch_ignore works within a locale *)
 crunch_ignore (add: bind)
 
 crunch crunch_foo9
-  for test': "\<lambda>x. x > y"
+  for test': "\<lambda>x. mstate x > y"
 
 end
 
@@ -200,7 +200,7 @@ end
 
 (* check that qualified names are handled properly. *)
 
-consts foo_const :: "(unit, unit) nondet_monad"
+consts foo_const :: "(unit, unit, unit) nondet_monad"
 defs foo_const_def: "foo_const \<equiv> Crunch_Test_Qualified_NonDet.foo_const"
 
 crunch foo_const
@@ -216,9 +216,9 @@ crunch crunch_foo3, crunch_foo4, crunch_foo5
 
 (* check that crunch can use wps to lift sub-predicates
    (and also that top-level constants can be ignored) *)
-consts crunch_foo11 :: "(nat, unit) nondet_monad"
-consts Q :: "bool \<Rightarrow> nat \<Rightarrow> bool"
-consts R :: "nat \<Rightarrow> bool"
+consts crunch_foo11 :: "(unit, nat, unit) nondet_monad"
+consts Q :: "bool \<Rightarrow> (unit, nat) monad_state \<Rightarrow> bool"
+consts R :: "(unit, nat) monad_state \<Rightarrow> bool"
 axiomatization
   where test1: "\<lbrace>Q x\<rbrace> crunch_foo11 \<lbrace>\<lambda>_. Q x\<rbrace>"
   and test2: "\<lbrace>\<lambda>s. P (R s)\<rbrace> crunch_foo11 \<lbrace>\<lambda>_ s. P (R s)\<rbrace>"
@@ -228,15 +228,17 @@ crunch crunch_foo11
   (wp: test1 wps: test2 ignore: crunch_foo11)
 
 (* check that crunch can handle functions lifted between different state spaces *)
-record 'a state =
+record 'a state = "unit monad_state_record" +
   state' :: nat
   ext :: 'a
 
-definition do_nat_op :: "(nat, unit) nondet_monad \<Rightarrow> ('a state,unit) nondet_monad" where
+type_synonym 'a state_x = "('a, unit) state_ext"
+
+definition do_nat_op :: "(unit, nat, unit) nondet_monad \<Rightarrow> (unit, 'a state_x, unit) nondet_monad" where
   "do_nat_op f \<equiv>
      do
        s \<leftarrow> get;
-       (_,s') \<leftarrow> select_f (mk_ef (f (state' s)));
+       (_, s') \<leftarrow> select_f (mk_ef (f (monad_state () (state' s))));
        modify (\<lambda>state. state\<lparr>state' := s'\<rparr>)
      od"
 
@@ -248,23 +250,23 @@ lemma do_nat_op_ef:
   done
 
 lemma nf_do_nat_op:
-  "no_fail P f \<Longrightarrow> empty_fail f \<Longrightarrow> no_fail (P \<circ> state') (do_nat_op f)"
+  "no_fail P f \<Longrightarrow> empty_fail f \<Longrightarrow> no_fail (P \<circ> monad_state () \<circ> state') (do_nat_op f)"
   unfolding do_nat_op_def
   apply wpsimp
   apply (fastforce simp: mk_ef_def no_fail_def empty_fail_def)
   done
 
 definition
-  "crunch_foo12_nat (x :: nat) = modify ((+) x)"
+  "crunch_foo12_nat (x :: nat) = modify (map_state ((+) x))"
 
-consts wrap_ext_op :: "(nat state, unit) nondet_monad \<Rightarrow> ('a state,unit) nondet_monad"
+consts wrap_ext_op :: "(unit, nat state_x, unit) nondet_monad \<Rightarrow> (unit, 'a state_x, unit) nondet_monad"
 consts unwrap_ext :: "'a state \<Rightarrow> nat state"
 
-definition do_extended_op :: "(nat state, unit) nondet_monad \<Rightarrow> ('a state,unit) nondet_monad" where
+definition do_extended_op :: "(unit, nat state_x, unit) nondet_monad \<Rightarrow> (unit, 'a state_x, unit) nondet_monad" where
   "do_extended_op eop \<equiv> do
                          ex \<leftarrow> get;
                          (_,es') \<leftarrow> select_f (mk_ef ((wrap_ext_op eop) ex));
-                         modify (\<lambda>state. state\<lparr>ext := (ext es')\<rparr>)
+                         modify (\<lambda>state. state\<lparr>ext := (ext (monad_state () es'))\<rparr>)
                         od"
 
 axiomatization
@@ -287,7 +289,7 @@ crunch crunch_foo12
   (wp: empty_fail_bind)
 
 (* check that other side conditions can still be collected when mixed with lifted functions*)
-definition crunch_foo13_pre :: "('a state,unit) nondet_monad" where
+definition crunch_foo13_pre :: "(unit, 'a state_x, unit) nondet_monad" where
   "crunch_foo13_pre \<equiv> return ()"
 
 axiomatization
